---
layout: post
title:  "Integral of \\(\\frac{1}{\\ln^2 x + 1}\\) (Ei + complex)"
date:   2023-03-07 20:28:00 -0600
categories: integrals
---

This integral came up while I was trying to integrate $$ \operatorname{atan}(\frac{1}{\ln x}) $$ (it's not that hard to see why). I'm still pretty new at solving integrals, but I'm thrilled to have learned a lesson here.

By the way, we're doing to be using this useful non-elementary function:

$$ \operatorname{Ei}(x) = \int \frac{e^x}{x}\,\mathrm dx $$

First, we do $$ u $$-substitution:

Let $$ u = \ln x $$, therefore $$ du = \frac{dx}{x} $$, and $$ e^u\,du = dx $$.

$$ \int \frac{1}{\ln^2 x + 1}\,\mathrm dx = \int \frac{e^u}{u^2 + 1}\,\mathrm du $$

I quickly got stuck here, until a friend (thanks Evan!) told me that this integral is not real. It's *complex*.

Sorry, you probably heard that joke a million times.

Going against my Algebra II teacher's advice that a sum of squares is not factorable, I went ahead and did it anyway only a year later.

$$ \int \frac{e^u}{(u + i)(u - i)}\,\mathrm du $$


By the way, you can't have exponents in the numerator during PFD. Not exactly sure why. It's no problem though, since we can separate the numerator from the denominator [as indicated by this helpful SE post.](https://math.stackexchange.com/questions/1047549/partial-fraction-decomposition-with-exponent-in-numerator)

$$ \int e^u\frac{1}{(u + i)(u - i)}\,\mathrm du $$

My deepest, darkest secret is that I despise partial fraction decomposition, but this one is easy.

$$ \frac{1}{(u + i)(u - i)} = \frac{A}{u + i} + \frac{B}{u - i} $$

$$ 1 = A(u - i) + B(u + i) $$

$$ A = -\frac{1}{2i}, B = \frac{1}{2i} $$

So

$$ \int \frac{e^u}{u^2 + 1}\,\mathrm du = \frac{1}{2i} \left[\int \frac{e^u}{u - i}\,\mathrm du - \int \frac{e^u}{u + i}\,\mathrm du\right] $$

Both of these integrals are non-elementary, but they're also pretty easy, thinking back to our $$ \operatorname{Ei}(x) $$ mentioned at the beginning of the post. I'll do one of them, but the other is evaluated the same way.

If we pick

$$ \int \frac{e^u}{u - i}\,\mathrm du $$

Let $$ w = u - i $$, then $$ u = w + i $$. It follows that

$$ \int \frac{e^{w + i}}{w}\,\mathrm dw = \int \frac{e^we^i}{w}\,\mathrm dw = e^i\int \frac{e^w}{w}\,\mathrm dw = e^i\operatorname{Ei}(w) = e^i\operatorname{Ei}(u - i) $$

We plug back in,

$$ \frac{1}{2i} \left[\int \frac{e^u}{u - i}\,\mathrm du - \int \frac{e^u}{u + i}\,\mathrm du\right] = \frac{e^i\operatorname{Ei}(u - i)}{2i} - \frac{e^{-i}\operatorname{Ei}(u + i)}{2i} $$

Substitute $$ u = \ln x $$ and add $$ +\:c $$ 

$$ \int \frac{1}{\ln^2 x + 1}\,\mathrm dx = \frac{e^i\operatorname{Ei}(\ln x - i)}{2i} - \frac{e^{-i}\operatorname{Ei}(\ln x + i)}{2i} + c $$

P.S. You might see some answers use the identity $$ \frac{1}{i} = -i $$.
